<?xml version="1.0"?>
<rdf:RDF
    xmlns:dul="http://www.ontologydesignpatterns.org/ont/dul/DUL.owl#"
    xmlns:rdf="http://www.w3.org/1999/02/22-rdf-syntax-ns#"
    xmlns:xsd="http://www.w3.org/2001/XMLSchema#"
    xmlns:rdfs="http://www.w3.org/2000/01/rdf-schema#"
    xmlns:owl="http://www.w3.org/2002/07/owl#"
    xmlns="http://www.ontologydesignpatterns.org/ont/dul/Conceptualization.owl#"
    xmlns:daml="http://www.daml.org/2001/03/daml+oil#"
  xml:base="http://www.ontologydesignpatterns.org/ont/dul/Conceptualization.owl">
  <owl:Ontology rdf:about="">
    <owl:imports rdf:resource="http://www.ontologydesignpatterns.org/ont/dul/DUL.owl"/>
    <rdfs:comment>A small set of patterns for representing different kinds of conceptualization relations between agents and social objects.</rdfs:comment>
    <owl:versionInfo rdf:datatype="http://www.w3.org/2001/XMLSchema#string"
    >0.1
Very preliminary as of now.
Author: Aldo Gangemi</owl:versionInfo>
  </owl:Ontology>
  <owl:Class rdf:ID="InternalRepresentation">
    <rdfs:label xml:lang="it">Rappresentazione interna</rdfs:label>
    <rdfs:label xml:lang="en">Internal representation</rdfs:label>
    <rdfs:subClassOf>
      <owl:Restriction>
        <owl:someValuesFrom>
          <owl:Restriction>
            <owl:someValuesFrom>
              <owl:Restriction>
                <owl:someValuesFrom rdf:resource="http://www.ontologydesignpatterns.org/ont/dul/DUL.owl#Agent"/>
                <owl:onProperty rdf:resource="http://www.ontologydesignpatterns.org/ont/dul/DUL.owl#isConceptualizedBy"/>
              </owl:Restriction>
            </owl:someValuesFrom>
            <owl:onProperty rdf:resource="http://www.ontologydesignpatterns.org/ont/dul/DUL.owl#expresses"/>
          </owl:Restriction>
        </owl:someValuesFrom>
        <owl:onProperty rdf:resource="http://www.ontologydesignpatterns.org/ont/dul/DUL.owl#realizes"/>
      </owl:Restriction>
    </rdfs:subClassOf>
    <rdfs:comment>The realization, within a cognitive system, of an information object expressing a social object conceptualized by that cognitive system.
For example, the subjective realization (within a human cognitive system) of some information expressing the meaning of Italian Traffic Law speed limits.</rdfs:comment>
    <rdfs:subClassOf rdf:resource="http://www.ontologydesignpatterns.org/ont/dul/DUL.owl#InformationRealization"/>
  </owl:Class>
  <owl:Class rdf:nodeID="A0">
    <owl:unionOf rdf:parseType="Collection">
      <rdf:Description rdf:about="http://www.ontologydesignpatterns.org/ont/dul/DUL.owl#Description"/>
      <rdf:Description rdf:about="http://www.ontologydesignpatterns.org/ont/dul/DUL.owl#Concept"/>
    </owl:unionOf>
  </owl:Class>
  <owl:Class rdf:nodeID="A1">
    <owl:unionOf rdf:parseType="Collection">
      <rdf:Description rdf:about="http://www.ontologydesignpatterns.org/ont/dul/DUL.owl#Description"/>
      <rdf:Description rdf:about="http://www.ontologydesignpatterns.org/ont/dul/DUL.owl#Concept"/>
    </owl:unionOf>
  </owl:Class>
  <owl:ObjectProperty rdf:ID="isKnownBy">
    <rdfs:subPropertyOf rdf:resource="http://www.ontologydesignpatterns.org/ont/dul/DUL.owl#isConceptualizedBy"/>
    <rdfs:domain rdf:resource="http://www.ontologydesignpatterns.org/ont/dul/DUL.owl#Situation"/>
    <rdfs:range rdf:resource="http://www.ontologydesignpatterns.org/ont/dul/DUL.owl#Agent"/>
    <owl:inverseOf>
      <owl:ObjectProperty rdf:ID="knows"/>
    </owl:inverseOf>
    <rdfs:label xml:lang="en">is known by</rdfs:label>
  </owl:ObjectProperty>
  <owl:ObjectProperty rdf:ID="isBelievedBy">
    <rdfs:subPropertyOf rdf:resource="http://www.ontologydesignpatterns.org/ont/dul/DUL.owl#isConceptualizedBy"/>
    <rdfs:domain rdf:resource="http://www.ontologydesignpatterns.org/ont/dul/DUL.owl#Situation"/>
    <rdfs:range rdf:resource="http://www.ontologydesignpatterns.org/ont/dul/DUL.owl#Agent"/>
    <owl:inverseOf>
      <owl:ObjectProperty rdf:ID="believes"/>
    </owl:inverseOf>
    <rdfs:label xml:lang="en">is believed by</rdfs:label>
  </owl:ObjectProperty>
  <owl:ObjectProperty rdf:ID="assumes">
    <rdfs:comment>An Agent assumes a (conceptualized) Description when she uses it to create a (mental) model or to draw inferences in some reasoning task. This is not the same as 'belief' in epistemic terms. Belief is about a Situation, considered as true, plausible, etc., while assumption is about assuming a Description or Concept.</rdfs:comment>
    <rdfs:domain rdf:resource="http://www.ontologydesignpatterns.org/ont/dul/DUL.owl#Agent"/>
    <rdfs:label xml:lang="it">assume</rdfs:label>
    <rdfs:subPropertyOf rdf:resource="http://www.ontologydesignpatterns.org/ont/dul/DUL.owl#conceptualizes"/>
    <owl:inverseOf>
      <owl:ObjectProperty rdf:ID="isAssumedBy"/>
    </owl:inverseOf>
    <rdfs:range rdf:nodeID="A1"/>
    <rdfs:label xml:lang="en">assumes</rdfs:label>
  </owl:ObjectProperty>
  <owl:ObjectProperty rdf:about="#isAssumedBy">
    <rdfs:domain rdf:nodeID="A1"/>
    <rdfs:label xml:lang="it">è assunto da</rdfs:label>
    <rdfs:comment>An Agent assumes a (conceptualized) Description when she uses it to create a (mental) model or to draw inferences in some reasoning task.</rdfs:comment>
    <owl:inverseOf rdf:resource="#assumes"/>
    <rdfs:subPropertyOf rdf:resource="http://www.ontologydesignpatterns.org/ont/dul/DUL.owl#isConceptualizedBy"/>
    <rdfs:range rdf:resource="http://www.ontologydesignpatterns.org/ont/dul/DUL.owl#Agent"/>
    <rdfs:label xml:lang="en">is assumed by</rdfs:label>
  </owl:ObjectProperty>
  <owl:ObjectProperty rdf:ID="isAdoptedBy">
    <rdfs:domain rdf:nodeID="A0"/>
    <rdfs:comment>An Agent adopts a Description when she assumes it in order to take Action or to devise a Plan</rdfs:comment>
    <owl:inverseOf>
      <owl:ObjectProperty rdf:ID="adopts"/>
    </owl:inverseOf>
    <rdfs:label xml:lang="it">è adottato da</rdfs:label>
    <rdfs:range rdf:resource="http://www.ontologydesignpatterns.org/ont/dul/DUL.owl#Agent"/>
    <rdfs:subPropertyOf rdf:resource="#isAssumedBy"/>
    <rdfs:label xml:lang="en">is adopted by</rdfs:label>
  </owl:ObjectProperty>
  <owl:ObjectProperty rdf:about="#adopts">
    <rdfs:range rdf:nodeID="A0"/>
    <rdfs:label xml:lang="it">adotta</rdfs:label>
    <owl:inverseOf rdf:resource="#isAdoptedBy"/>
    <rdfs:comment>An Agent adopts a Description or a Concept when she assumes it in order to take Action or to devise a Plan. In this case, the assumption is stronger, because the Agent wants to commit to some world-changing action on the basis of a Description. This is still different from believes, which concerns epistemic attitude towards a Situation.</rdfs:comment>
    <rdfs:domain rdf:resource="http://www.ontologydesignpatterns.org/ont/dul/DUL.owl#Agent"/>
    <rdfs:subPropertyOf rdf:resource="#assumes"/>
    <rdfs:label xml:lang="en">adopts</rdfs:label>
  </owl:ObjectProperty>
  <owl:ObjectProperty rdf:about="#believes">
    <rdfs:label xml:lang="it">crede</rdfs:label>
    <rdfs:comment>The conceptualization of a Situation that is only indirectly perceived and processed by an Agent</rdfs:comment>
    <owl:inverseOf rdf:resource="#isBelievedBy"/>
    <rdfs:range rdf:resource="http://www.ontologydesignpatterns.org/ont/dul/DUL.owl#Situation"/>
    <rdfs:domain rdf:resource="http://www.ontologydesignpatterns.org/ont/dul/DUL.owl#Agent"/>
    <rdfs:subPropertyOf rdf:resource="http://www.ontologydesignpatterns.org/ont/dul/DUL.owl#conceptualizes"/>
    <rdfs:label xml:lang="en">believes</rdfs:label>
  </owl:ObjectProperty>
  <owl:ObjectProperty rdf:about="#knows">
    <rdfs:label xml:lang="it">sa</rdfs:label>
    <rdfs:comment>The conceptualization of a Situation perceived and processed with 'certainty' by an Agent</rdfs:comment>
    <owl:inverseOf rdf:resource="#isKnownBy"/>
    <rdfs:range rdf:resource="http://www.ontologydesignpatterns.org/ont/dul/DUL.owl#Situation"/>
    <rdfs:domain rdf:resource="http://www.ontologydesignpatterns.org/ont/dul/DUL.owl#Agent"/>
    <rdfs:subPropertyOf rdf:resource="http://www.ontologydesignpatterns.org/ont/dul/DUL.owl#conceptualizes"/>
    <rdfs:label xml:lang="en">knows</rdfs:label>
  </owl:ObjectProperty>
  <rdf:Description rdf:about="http://www.ontologydesignpatterns.org/ont/dul/DUL.owl#actsThrough">
    <rdfs:range rdf:resource="http://www.ontologydesignpatterns.org/ont/dul/DUL.owl#Agent"/>
  </rdf:Description>
</rdf:RDF>
