@prefix : <https://loted2.googlecode.com/svn/trunk/modules/ProcurementsTopClasses#> .
@prefix dc: <http://purl.org/dc/terms/> .
@prefix owl: <http://www.w3.org/2002/07/owl#> .
@prefix rdf: <http://www.w3.org/1999/02/22-rdf-syntax-ns#> .
@prefix xml: <http://www.w3.org/XML/1998/namespace> .
@prefix xsd: <http://www.w3.org/2001/XMLSchema#> .
@prefix rdfs: <http://www.w3.org/2000/01/rdf-schema#> .
@prefix ProcurementsTopClasses: <https://loted2.googlecode.com/svn/trunk/modules/ProcurementsTopClasses#> .
@base <https://loted2.googlecode.com/svn/trunk/modules/ProcurementsTopClasses> .

<https://loted2.googlecode.com/svn/trunk/modules/ProcurementsTopClasses> rdf:type owl:Ontology ;
                                                                          owl:versionIRI <https://loted2.googlecode.com/svn/trunk/modules/ProcurementsTopClasses> ;
                                                                          dc:contributor "Enrico Motta"^^xsd:string ,
                                                                                         "Mathieu d'Aquin"^^xsd:string ;
                                                                          dc:creator "Isabella Distinto" ;
                                                                          dc:date "2013-07-24" ;
                                                                          dc:description "The ontology was created by Isabella Distinto, with input from Mathieu d'Aquin and Enrico Motta."^^xsd:string ;
                                                                          dc:language "en"^^xsd:language ;
                                                                          dc:title "LOTED2: Procurements Top Classes Module"^^xsd:string ;
                                                                          rdfs:comment "The Procurements Top Classes is the upper module of LOTED2 ontology and is meant to represent the most abstract and general classes related to the public procurement domain. The classes of this module are represented with the purpose to allow mappings between LOTED2 ontology and other ontologies. Consistently with such an aim, many classes of the Procurements Top Classes module have been modeled by reusing the Legal Knowledge Interchange Format (LKIF) ontology (see: http://www.estrellaproject.org/lkif-core/) as a source of patterns."@en ;
                                                                          rdfs:label "LOTED2: Procurements Top Module" ,
                                                                                     "Procurements Top Classes Definition"@en ;
                                                                          owl:versionInfo "2.0"@en .

#################################################################
#    Annotation properties
#################################################################

###  http://purl.org/dc/terms/contributor
dc:contributor rdf:type owl:AnnotationProperty .


###  http://purl.org/dc/terms/creator
dc:creator rdf:type owl:AnnotationProperty .


###  http://purl.org/dc/terms/date
dc:date rdf:type owl:AnnotationProperty .


###  http://purl.org/dc/terms/description
dc:description rdf:type owl:AnnotationProperty .


###  http://purl.org/dc/terms/language
dc:language rdf:type owl:AnnotationProperty .


###  http://purl.org/dc/terms/title
dc:title rdf:type owl:AnnotationProperty .


###  http://www.w3.org/2000/01/rdf-schema#comment
rdfs:comment rdf:type owl:AnnotationProperty .


###  http://www.w3.org/2000/01/rdf-schema#label
rdfs:label rdf:type owl:AnnotationProperty .


###  http://www.w3.org/2002/07/owl#versionInfo
owl:versionInfo rdf:type owl:AnnotationProperty .


#################################################################
#    Object Properties
#################################################################

###  https://loted2.googlecode.com/svn/trunk/modules/ProcurementsTopClasses#contactPoint
ProcurementsTopClasses:contactPoint rdf:type owl:ObjectProperty ;
                                    rdfs:domain [ rdf:type owl:Class ;
                                                  owl:unionOf ( ProcurementsTopClasses:NaturalPerson
                                                                ProcurementsTopClasses:Organisation
                                                                ProcurementsTopClasses:OrganisationalUnit
                                                              )
                                                ] ;
                                    rdfs:range ProcurementsTopClasses:VCard ;
                                    rdfs:comment "The contact point of a person or an organisation or an organisational unit defined with VCard ontology (http://www.w3.org/2006/vcard/ns)."@en ;
                                    rdfs:label "contact point (1..*)"@en .


###  https://loted2.googlecode.com/svn/trunk/modules/ProcurementsTopClasses#context
ProcurementsTopClasses:context rdf:type owl:ObjectProperty ;
                               rdfs:domain ProcurementsTopClasses:Role ;
                               rdfs:range [ rdf:type owl:Class ;
                                            owl:unionOf ( ProcurementsTopClasses:Organisation
                                                          ProcurementsTopClasses:Process
                                                        )
                                          ] ;
                               rdfs:comment "The context (process or organisation) in which a role is played by an agent."@en ;
                               rdfs:label "context (1..1)"@en .


###  https://loted2.googlecode.com/svn/trunk/modules/ProcurementsTopClasses#hasActivity
ProcurementsTopClasses:hasActivity rdf:type owl:ObjectProperty ;
                                   owl:inverseOf ProcurementsTopClasses:isActivityOf ;
                                   rdfs:domain ProcurementsTopClasses:Agent ;
                                   rdfs:range ProcurementsTopClasses:Activity ;
                                   rdfs:comment "The activity carried out by a person or an organisation."@en ;
                                   rdfs:label "has activity (0..*)"@en .


###  https://loted2.googlecode.com/svn/trunk/modules/ProcurementsTopClasses#hasAuthor
ProcurementsTopClasses:hasAuthor rdf:type owl:ObjectProperty ;
                                 owl:inverseOf ProcurementsTopClasses:isAuthorOf ;
                                 rdfs:domain ProcurementsTopClasses:Document ;
                                 rdfs:range ProcurementsTopClasses:Agent ;
                                 rdfs:comment "The document has an agent as author."@en ;
                                 rdfs:label "has author (0..*)"@en .


###  https://loted2.googlecode.com/svn/trunk/modules/ProcurementsTopClasses#hasCountry
ProcurementsTopClasses:hasCountry rdf:type owl:ObjectProperty ;
                                  rdfs:domain ProcurementsTopClasses:Agent ;
                                  rdfs:range ProcurementsTopClasses:Country ;
                                  rdfs:comment """This property mainly aims to connect the class LOTED2:Agent with the LOTED2: Country in which is located. 

This information is relevant to determine what kind of regulation (i.e. LOTED2: LegislativeSource) has to be applied to the tender. For example: if a LOTED2: PublicUndertaking hasCountry LOTED2: IT (Italy, that is an EU member State), then the LOTED2: ContractNotice announced by this contracting authority must be respectful of EC Directives, and also of the specific national legislation that implements the Directives (in the case of Italy the D. Lgs. n. 163/2006).

The place of performance of contract is normally defined with the name of a city (obviously located in a country), and it is also possible to infer this place through the NUTS code, because the first two letters of this code represent the country in which the place is located. 

Note: is not clear whether the raw data of the TED refers to the country of the awarding authority or to the place of performance of contract. 
"""@en ;
                                  rdfs:label "hasCountry (1..1)"@en .


###  https://loted2.googlecode.com/svn/trunk/modules/ProcurementsTopClasses#isActivityOf
ProcurementsTopClasses:isActivityOf rdf:type owl:ObjectProperty ;
                                    rdfs:domain ProcurementsTopClasses:Activity ;
                                    rdfs:range ProcurementsTopClasses:Agent ;
                                    rdfs:label "is activity of (0..*)"@en .


###  https://loted2.googlecode.com/svn/trunk/modules/ProcurementsTopClasses#isAuthorOf
ProcurementsTopClasses:isAuthorOf rdf:type owl:ObjectProperty ;
                                  rdfs:comment "The author of a document."@en ;
                                  rdfs:label "is author of (0..*)"@en .


###  https://loted2.googlecode.com/svn/trunk/modules/ProcurementsTopClasses#legalContext
ProcurementsTopClasses:legalContext rdf:type owl:ObjectProperty ;
                                    rdfs:subPropertyOf ProcurementsTopClasses:context ;
                                    rdfs:domain ProcurementsTopClasses:LegalRole ;
                                    rdfs:comment "The legal context in which a legal role is palyed by a natural or legal person."@en ;
                                    rdfs:label "legal context (1..1)"@en .


###  https://loted2.googlecode.com/svn/trunk/modules/ProcurementsTopClasses#member
ProcurementsTopClasses:member rdf:type owl:ObjectProperty ;
                              owl:inverseOf ProcurementsTopClasses:memberOf ;
                              rdfs:domain ProcurementsTopClasses:Organisation ;
                              rdfs:range [ rdf:type owl:Class ;
                                           owl:unionOf ( ProcurementsTopClasses:NaturalPerson
                                                         ProcurementsTopClasses:Organisation
                                                       )
                                         ] ;
                              rdfs:comment "This property specifies membership of an organisation."@en ;
                              rdfs:label "member (1..*)"@en .


###  https://loted2.googlecode.com/svn/trunk/modules/ProcurementsTopClasses#memberOf
ProcurementsTopClasses:memberOf rdf:type owl:ObjectProperty ;
                                rdfs:label "member of (1..*)"@en .


###  https://loted2.googlecode.com/svn/trunk/modules/ProcurementsTopClasses#playsLegalRoleIn
ProcurementsTopClasses:playsLegalRoleIn rdf:type owl:ObjectProperty ;
                                        rdfs:subPropertyOf ProcurementsTopClasses:playsRoleIn ;
                                        rdfs:domain [ rdf:type owl:Class ;
                                                      owl:unionOf ( ProcurementsTopClasses:LegalPerson
                                                                    ProcurementsTopClasses:NaturalPerson
                                                                  )
                                                    ] ;
                                        rdfs:range [ rdf:type owl:Class ;
                                                     owl:unionOf ( ProcurementsTopClasses:Organisation
                                                                   ProcurementsTopClasses:Process
                                                                 )
                                                   ] ;
                                        owl:propertyChainAxiom ( ProcurementsTopClasses:playsRole
                                                                 ProcurementsTopClasses:legalContext
                                                               ) ;
                                        rdfs:comment "The legal context in which a natural person or a legal person plays a legal role."@en ;
                                        rdfs:label "plays legal role in (1..1)"@en .


###  https://loted2.googlecode.com/svn/trunk/modules/ProcurementsTopClasses#playsRole
ProcurementsTopClasses:playsRole rdf:type owl:ObjectProperty ;
                                 owl:inverseOf ProcurementsTopClasses:rolePlayedBy ;
                                 rdfs:domain ProcurementsTopClasses:Agent ;
                                 rdfs:range ProcurementsTopClasses:Role ;
                                 rdfs:comment "The role that an agent may play in a context."@en ;
                                 rdfs:label "plays role (0..*)"@en .


###  https://loted2.googlecode.com/svn/trunk/modules/ProcurementsTopClasses#playsRoleIn
ProcurementsTopClasses:playsRoleIn rdf:type owl:ObjectProperty ;
                                   rdfs:domain ProcurementsTopClasses:Agent ;
                                   rdfs:range [ rdf:type owl:Class ;
                                                owl:unionOf ( ProcurementsTopClasses:Organisation
                                                              ProcurementsTopClasses:Process
                                                            )
                                              ] ;
                                   owl:propertyChainAxiom ( ProcurementsTopClasses:playsRole
                                                            ProcurementsTopClasses:context
                                                          ) ;
                                   rdfs:comment "The context in which an agent plays a role."@en ;
                                   rdfs:label "plays role in (1..1)"@en .


###  https://loted2.googlecode.com/svn/trunk/modules/ProcurementsTopClasses#rolePlayedBy
ProcurementsTopClasses:rolePlayedBy rdf:type owl:ObjectProperty ;
                                    rdfs:domain ProcurementsTopClasses:Role ;
                                    rdfs:range ProcurementsTopClasses:Agent ;
                                    rdfs:label "role played by (0..*)"@en .


#################################################################
#    Classes
#################################################################

###  http://www.w3.org/2002/07/owl#Thing
owl:Thing rdf:type owl:Class .


###  https://loted2.googlecode.com/svn/trunk/modules/ProcurementsTopClasses#Activity
ProcurementsTopClasses:Activity rdf:type owl:Class ;
                                rdfs:subClassOf ProcurementsTopClasses:Process ;
                                rdfs:comment "The class of activities carried out by organizations or individuals."@en ;
                                rdfs:label "Activity"@en .


###  https://loted2.googlecode.com/svn/trunk/modules/ProcurementsTopClasses#AdministrativeDocument
ProcurementsTopClasses:AdministrativeDocument rdf:type owl:Class ;
                                              rdfs:subClassOf ProcurementsTopClasses:LegalDocument ;
                                              rdfs:comment """An administrative document is a document issued by an entity in order to carry out an administrative function. 

Note that administrative documents can be drafted also by private legal entities and not only by public bodies. 
This is the case, for example, of the conctract notice issued by the public works concessionaire."""@en ;
                                              rdfs:label "Administrative document"@en .


###  https://loted2.googlecode.com/svn/trunk/modules/ProcurementsTopClasses#Agent
ProcurementsTopClasses:Agent rdf:type owl:Class ;
                             owl:disjointWith ProcurementsTopClasses:Country ,
                                              ProcurementsTopClasses:Document ,
                                              ProcurementsTopClasses:Language ,
                                              ProcurementsTopClasses:LegalSource ,
                                              ProcurementsTopClasses:Location ,
                                              ProcurementsTopClasses:Process ,
                                              ProcurementsTopClasses:Role ;
                             rdfs:comment "Any agent, either natural or legal person, individual or social (e.g. an organisation, a corporation, an institution)."@en ;
                             rdfs:label "Agent"@en .


###  https://loted2.googlecode.com/svn/trunk/modules/ProcurementsTopClasses#Code
ProcurementsTopClasses:Code rdf:type owl:Class ;
                            rdfs:subClassOf ProcurementsTopClasses:LegislativeDocument ;
                            owl:disjointWith ProcurementsTopClasses:Directive ,
                                             ProcurementsTopClasses:InternationalAgreement ;
                            rdfs:comment "A code is a type of legislation that purports to exhaustively cover a complete system of laws or a particular area of law as it existed at the time the code was enacted, by a process of codification. (Source: Wikipedia)."@en ;
                            rdfs:label "Code"@en .


###  https://loted2.googlecode.com/svn/trunk/modules/ProcurementsTopClasses#Country
ProcurementsTopClasses:Country rdf:type owl:Class ;
                               owl:disjointWith ProcurementsTopClasses:Document ,
                                                ProcurementsTopClasses:Language ,
                                                ProcurementsTopClasses:LegalSource ,
                                                ProcurementsTopClasses:Location ,
                                                ProcurementsTopClasses:Process ;
                               rdfs:comment "A country is a region legally identified as a distinct entity in political geography (Source: Wikipedia)."@en ;
                               rdfs:label "Country"@en .


###  https://loted2.googlecode.com/svn/trunk/modules/ProcurementsTopClasses#Directive
ProcurementsTopClasses:Directive rdf:type owl:Class ;
                                 rdfs:subClassOf ProcurementsTopClasses:LegislativeDocument ;
                                 owl:disjointWith ProcurementsTopClasses:InternationalAgreement ;
                                 rdfs:comment "Examples are European Union directives, which are legislative acts of the European Union and Directives, used by United States Government agencies (particularly the Department of Defense) to convey policies, responsibilities, and procedures (Source: LKIF-Core ontology)."@en ;
                                 rdfs:label "Directive"@en .


###  https://loted2.googlecode.com/svn/trunk/modules/ProcurementsTopClasses#Document
ProcurementsTopClasses:Document rdf:type owl:Class ;
                                owl:disjointWith ProcurementsTopClasses:Language ,
                                                 ProcurementsTopClasses:Location ,
                                                 ProcurementsTopClasses:Process ;
                                rdfs:comment """A Document bears some (and only) expression(s) stated by some statement in writing (Source: LKIF-Core ontology).
This class is equivalent to foaf: Document."""@en ;
                                rdfs:label "Document"@en .


###  https://loted2.googlecode.com/svn/trunk/modules/ProcurementsTopClasses#EEACountry
ProcurementsTopClasses:EEACountry rdf:type owl:Class ;
                                  rdfs:subClassOf ProcurementsTopClasses:Country ;
                                  rdfs:comment "The 28 EU Member States and the three EEA EFTA States (Iceland, Liechtenstein and Norway). Switzerland is not part of the EEA Agreement, but has a bilateral agreement with the EU."@en ;
                                  rdfs:label "EEA country"@en .


###  https://loted2.googlecode.com/svn/trunk/modules/ProcurementsTopClasses#EUMember
ProcurementsTopClasses:EUMember rdf:type owl:Class ;
                                rdfs:subClassOf ProcurementsTopClasses:Country ;
                                rdfs:comment "The 28 EU Member States of the EU (Austria, Belgium, Bulgaria, Croatia, Cyprus, Czech Republic, Denmark, Estonia, Finland, France, Germany, Greece, Hungary, Ireland, Italy, Latvia, Lithuania, Luxembourg, Malta, Netherlands, Poland, Portugal, Romania, Slovakia, Slovenia, Spain, Sweden, United Kingdom)."@en ;
                                rdfs:label "EU member"@en .


###  https://loted2.googlecode.com/svn/trunk/modules/ProcurementsTopClasses#EUOfficialLanguage
ProcurementsTopClasses:EUOfficialLanguage rdf:type owl:Class ;
                                          rdfs:subClassOf ProcurementsTopClasses:Language ;
                                          owl:disjointWith ProcurementsTopClasses:NonEUOfficialLanguage ;
                                          rdfs:comment "Any official language of the European Union."@en ;
                                          rdfs:label "EU official language"@en .


###  https://loted2.googlecode.com/svn/trunk/modules/ProcurementsTopClasses#Function
ProcurementsTopClasses:Function rdf:type owl:Class ;
                                rdfs:subClassOf ProcurementsTopClasses:Role ;
                                rdfs:comment "The use or purpose of some object as used in some context (Source: LKIF-core ontology)."@en ;
                                rdfs:label "Function"@en .


###  https://loted2.googlecode.com/svn/trunk/modules/ProcurementsTopClasses#GPACountry
ProcurementsTopClasses:GPACountry rdf:type owl:Class ;
                                  rdfs:subClassOf ProcurementsTopClasses:Country ;
                                  rdfs:comment "Any country which is party to the Government Procurement Agreement."@en ;
                                  rdfs:label "GPA Country"@en .


###  https://loted2.googlecode.com/svn/trunk/modules/ProcurementsTopClasses#InternationalAgreement
ProcurementsTopClasses:InternationalAgreement rdf:type owl:Class ;
                                              rdfs:subClassOf ProcurementsTopClasses:LegalSource ,
                                                              ProcurementsTopClasses:SourceOfInternationalLaw ;
                                              rdfs:comment "An agreement entered into by actors in international law, namely states and international organizations (Source: LKIF-Core ontology)."@en ;
                                              rdfs:label "International agreement"@en .


###  https://loted2.googlecode.com/svn/trunk/modules/ProcurementsTopClasses#Language
ProcurementsTopClasses:Language rdf:type owl:Class ;
                                owl:disjointWith ProcurementsTopClasses:LegalSource ,
                                                 ProcurementsTopClasses:Location ,
                                                 ProcurementsTopClasses:Process ;
                                rdfs:comment "The class of languages."@en ;
                                rdfs:label "Language"@en .


###  https://loted2.googlecode.com/svn/trunk/modules/ProcurementsTopClasses#LegalDocument
ProcurementsTopClasses:LegalDocument rdf:type owl:Class ;
                                     rdfs:subClassOf ProcurementsTopClasses:Document ,
                                                     ProcurementsTopClasses:LegalSource ;
                                     rdfs:comment "A legal document is a document bearing norms or normative statements (Source: LKIF-Core ontology)."@en ;
                                     rdfs:label "Legal document"@en .


###  https://loted2.googlecode.com/svn/trunk/modules/ProcurementsTopClasses#LegalPerson
ProcurementsTopClasses:LegalPerson rdf:type owl:Class ;
                                   rdfs:subClassOf ProcurementsTopClasses:Organisation ;
                                   rdfs:comment """A legal entity is a natural person or a legal construct through which the law allows a group of natural persons to act as if it were a single composite individual for certain purposes. The most common purposes are lawsuits, property ownership, and contracts. Sometimes referred to as corporate personhood or legal personality, this concept allows for easy conduct of business by having ownership, lawsuits, and agreements under the name of the legal entity instead of the several names of the people making up the entity.

A legal entity is not necessarily distinct from the natural persons of which it is composed. Most legal entities are simply amalgamations of the persons that make it up for convenience's sake. A legal entity that does have a separate existence from its members is called a company or corporation. This distinction gives the corporation its unique perpetual succession privilege and is usually also the source of the limited liability of corporate members. Some other legal entities also enjoy limited liability of members, but not on account of separate existence (Source: Wikipedia.org)."""@en ;
                                   rdfs:label "Legal person"@en .


###  https://loted2.googlecode.com/svn/trunk/modules/ProcurementsTopClasses#LegalRole
ProcurementsTopClasses:LegalRole rdf:type owl:Class ;
                                 rdfs:subClassOf ProcurementsTopClasses:Role ;
                                 rdfs:comment "A legal role is a role played in a legal context. Legal role players can be both Agents and other 'things' (Source: LKIF-core ontology)."@en ;
                                 rdfs:label "Legal role"@en .


###  https://loted2.googlecode.com/svn/trunk/modules/ProcurementsTopClasses#LegalSource
ProcurementsTopClasses:LegalSource rdf:type owl:Class ;
                                   owl:disjointWith ProcurementsTopClasses:Location ,
                                                    ProcurementsTopClasses:OrganisationalUnit ,
                                                    ProcurementsTopClasses:Process ;
                                   rdfs:comment "Any source of law."@en ;
                                   rdfs:label "Legal source"@en .


###  https://loted2.googlecode.com/svn/trunk/modules/ProcurementsTopClasses#LegislativeDocument
ProcurementsTopClasses:LegislativeDocument rdf:type owl:Class ;
                                           rdfs:subClassOf ProcurementsTopClasses:LegalDocument ,
                                                           ProcurementsTopClasses:LegislativeSource ;
                                           rdfs:comment "A legal document that contains norms and is drafted by a public body with legislative power (for example the Parliament) in order to regulate general and abstract situations."@en ;
                                           rdfs:label "Legislative document"@en .


###  https://loted2.googlecode.com/svn/trunk/modules/ProcurementsTopClasses#LegislativeSource
ProcurementsTopClasses:LegislativeSource rdf:type owl:Class ;
                                         rdfs:subClassOf ProcurementsTopClasses:LegalSource ;
                                         rdfs:comment "Any legislative document which is a source of law."@en ;
                                         rdfs:label "Legislative source"@en .


###  https://loted2.googlecode.com/svn/trunk/modules/ProcurementsTopClasses#Location
ProcurementsTopClasses:Location rdf:type owl:Class ;
                                owl:disjointWith ProcurementsTopClasses:Process ;
                                rdfs:comment "The terms location and place in geography are used to notice and or identify a point or an area on the Earth's surface or elsewhere. The term 'location' generally implies a higher degree of certainty than \"place\" which often has an ambiguous boundary relying more on human/social attributes of place identity and sense of place than on geometry (Source: Wikipedia)."@en ;
                                rdfs:label "Location"@en .


###  https://loted2.googlecode.com/svn/trunk/modules/ProcurementsTopClasses#NaturalPerson
ProcurementsTopClasses:NaturalPerson rdf:type owl:Class ;
                                     rdfs:subClassOf ProcurementsTopClasses:Agent ;
                                     rdfs:comment """A person is an individual agent. Usually associated with 'human being'(Source: LKIF-Core ontology).
This class is equivalent to foaf: Person."""@en ;
                                     rdfs:label "Natural person"@en .


###  https://loted2.googlecode.com/svn/trunk/modules/ProcurementsTopClasses#NonEUOfficialLanguage
ProcurementsTopClasses:NonEUOfficialLanguage rdf:type owl:Class ;
                                             rdfs:subClassOf ProcurementsTopClasses:Language ;
                                             rdfs:comment "Any language which is not an EU offical languages."@en ;
                                             rdfs:label "NonEUOfficialLanguage"@en .


###  https://loted2.googlecode.com/svn/trunk/modules/ProcurementsTopClasses#Organisation
ProcurementsTopClasses:Organisation rdf:type owl:Class ;
                                    rdfs:subClassOf ProcurementsTopClasses:Agent ,
                                                    [ rdf:type owl:Restriction ;
                                                      owl:onProperty ProcurementsTopClasses:member ;
                                                      owl:allValuesFrom [ rdf:type owl:Class ;
                                                                          owl:unionOf ( ProcurementsTopClasses:NaturalPerson
                                                                                        ProcurementsTopClasses:Organisation
                                                                                      )
                                                                        ]
                                                    ] ;
                                    rdfs:comment """An organisation is a group of other organisations or persons which acts 'as one'. An organisation can be both formal (i.e. created by law or decree) or informal (Source: LKIF-Core ontology).

This class is equivalent to foaf: Organisation."""@en ;
                                    rdfs:label "Organisation"@en .


###  https://loted2.googlecode.com/svn/trunk/modules/ProcurementsTopClasses#OrganisationalUnit
ProcurementsTopClasses:OrganisationalUnit rdf:type owl:Class ;
                                          rdfs:subClassOf owl:Thing ;
                                          rdfs:comment """'The name \"Organizational Unit\" appears to represent a single organization with multiple units (departments) within that organization.' (Source: Wikipedia)

An organisation unit may be of different types such as department, divisions, etc. on the basis of the organisation chart.

In the LOTED2 ontology this class is important because some contracting authorities/entities may have several organisational units, which are deputed to give information about the tender or to provide specifications and additional documents, or to receive tenders and requests to participate to a tender. 

Since that these organisational units can be deployed in different places, they may have their own address other than this of the Organization they belong. This can be represented with VCard vocabulary. Note that the datatype property vcard: organisation-unit is in this ontology equivalent to LOTED2: organisationalUnit-name, that define the name of the ted: OrganisationalUnit."""@en ;
                                          rdfs:label "Organisational unit"@en .


###  https://loted2.googlecode.com/svn/trunk/modules/ProcurementsTopClasses#PrivateLegalPerson
ProcurementsTopClasses:PrivateLegalPerson rdf:type owl:Class ;
                                          rdfs:subClassOf ProcurementsTopClasses:LegalPerson ;
                                          rdfs:comment "'A legal person as defined in private law' (Source: LKIF-Core ontology)."@en ;
                                          rdfs:label "Private legal person"@en .


###  https://loted2.googlecode.com/svn/trunk/modules/ProcurementsTopClasses#Process
ProcurementsTopClasses:Process rdf:type owl:Class ;
                               rdfs:comment "'A series of actions or steps taken in order to achieve a particular end' (Source: Oxford dictionary)."@en ;
                               rdfs:label "Process"@en .


###  https://loted2.googlecode.com/svn/trunk/modules/ProcurementsTopClasses#PublicBody
ProcurementsTopClasses:PublicBody rdf:type owl:Class ;
                                  rdfs:subClassOf ProcurementsTopClasses:LegalPerson ;
                                  rdfs:comment "'A public body or body created by an act of law to serve a public interest' (Source: LKIF-Core ontology)."@en ;
                                  rdfs:label "Public body"@en .


###  https://loted2.googlecode.com/svn/trunk/modules/ProcurementsTopClasses#Role
ProcurementsTopClasses:Role rdf:type owl:Class ;
                            rdfs:comment "A role is a specification of default behavior and accompanying expectations of the thing 'playing' the role. Similar to actors in a theater who play roles, but are not the roles. Example: student (Source: LKIF-core ontology)."@en ;
                            rdfs:label "Role"@en .


###  https://loted2.googlecode.com/svn/trunk/modules/ProcurementsTopClasses#SourceOfInternationalLaw
ProcurementsTopClasses:SourceOfInternationalLaw rdf:type owl:Class ;
                                                rdfs:subClassOf ProcurementsTopClasses:LegalSource ;
                                                rdfs:comment "Any source of International law such as International agreements, treaty, etc."@en ;
                                                rdfs:label "Source of international law"@en .


###  https://loted2.googlecode.com/svn/trunk/modules/ProcurementsTopClasses#VCard
ProcurementsTopClasses:VCard rdf:type owl:Class ;
                             rdfs:comment "vCard is a file format standard for electronic business cards."@en ;
                             rdfs:label "VCard"@en .


###  Generated by the OWL API (version 4.5.9.2019-02-01T07:24:44Z) https://github.com/owlcs/owlapi
